decidability of isgPartsC

type/decidability.v
@@ -1,9 +1,381 @@
-From SST Require Export type.global type.local type.isomorphism type.projection type.merge.
-Require Import List String Datatypes ZArith Relations PeanoNat. 
-Open Scope list_scope.
+From mathcomp Require Import ssreflect.seq all_ssreflect.
 From Paco Require Import paco pacotac.
-Require Import Setoid Morphisms Coq.Program.Basics.
-Require Import Coq.Init.Datatypes Coq.Logic.Decidable.
+From SST Require Export src.expressions src.header type.global type.local type.isomorphism type.merge.
+Require Import List String Coq.Arith.PeanoNat Relations Coq.Logic.Decidable.
+Import ListNotations. 
+
+Inductive isgParts : part -> global -> Prop := 
+  | pa_sendp : forall p q l, isgParts p (g_send p q l)
+  | pa_sendq : forall p q l, isgParts q (g_send p q l)
+  | pa_mu    : forall p g,   isgParts p g -> isgParts p (g_rec g)
+  | pa_sendr : forall p q r n s g lis, p <> r -> q <> r -> onth n lis = Some (s, g) -> isgParts r g -> isgParts r (g_send p q lis).
+  
+Definition isgPartsC (pt : part) (G : gtt) : Prop := 
+    exists G', gttTC G' G /\ (forall n, exists m, guardG n m G') /\ isgParts pt G'.
+
+Inductive ishParts : part -> gtth -> Prop := 
+  | ha_sendp : forall p q l, ishParts p (gtth_send p q l)
+  | ha_sendq : forall p q l, ishParts q (gtth_send p q l)
+  | ha_sendr : forall p q r n s g lis, p <> r -> q <> r -> onth n lis = Some (s, g) -> ishParts r g -> ishParts r (gtth_send p q lis).
+
+
+Lemma triv_pt_p : forall p q x0,
+    wfgC (gtt_send p q x0) -> 
+    isgPartsC p (gtt_send p q x0).
+Proof.
+  intros. unfold wfgC in H.
+  destruct H. destruct H. destruct H0. destruct H1.
+  unfold isgPartsC in *.
+  pinversion H; try easy. 
+  - subst. exists (g_send p q xs). split. pfold. easy. split. easy. constructor.
+  - subst. specialize(guard_breakG G H1); intros. 
+    destruct H5. destruct H5. destruct H6.
+   
+    destruct H7.
+    - subst. 
+      specialize(gttTC_after_subst (g_rec G) g_end (gtt_send p q x0) H5); intros.
+      assert(gttTC g_end (gtt_send p q x0)). 
+      apply H7. pfold. easy. pinversion H8. 
+      apply gttT_mon.
+    destruct H7. destruct H7. destruct H7.
+    - subst.
+      specialize(gttTC_after_subst (g_rec G) (g_send x1 x2 x3) (gtt_send p q x0) H5); intros.
+      assert(gttTC (g_send x1 x2 x3) (gtt_send p q x0)).
+      apply H7. pfold. easy.
+      pinversion H8. subst.
+      exists (g_send p q x3). split; try easy. pfold. easy. split. easy.
+      constructor.
+    apply gttT_mon.
+    apply gttT_mon.
+Qed.
+
+
+Lemma triv_pt_q : forall p q x0,
+    wfgC (gtt_send p q x0) -> 
+    isgPartsC q (gtt_send p q x0).
+Proof.
+  intros. unfold wfgC in H.
+  destruct H. destruct H. destruct H0. destruct H1.
+  unfold isgPartsC in *.
+  pinversion H; try easy. 
+  - subst. exists (g_send p q xs). split. pfold. easy. constructor. easy. constructor.
+  - subst. specialize(guard_breakG G H1); intros. 
+    destruct H5. destruct H5. destruct H6.
+   
+    destruct H7.
+    - subst. 
+      specialize(gttTC_after_subst (g_rec G) g_end (gtt_send p q x0) H5); intros.
+      assert(gttTC g_end (gtt_send p q x0)). 
+      apply H7. pfold. easy. pinversion H8. 
+      apply gttT_mon.
+    destruct H7. destruct H7. destruct H7.
+    - subst.
+      specialize(gttTC_after_subst (g_rec G) (g_send x1 x2 x3) (gtt_send p q x0) H5); intros.
+      assert(gttTC (g_send x1 x2 x3) (gtt_send p q x0)).
+      apply H7. pfold. easy.
+      pinversion H8. subst.
+      exists (g_send p q x3). split; try easy. pfold. easy. 
+      split. easy. constructor.
+    apply gttT_mon.
+    apply gttT_mon.
+Qed.
+
+
+Lemma ishParts_x : forall [p s1 s2 o1 o2 xs0],
+    (ishParts p (gtth_send s1 s2 (Some (o1,o2) :: xs0)) -> False) ->
+    (ishParts p o2 -> False).
+Proof.
+  intros. apply H. 
+  - case_eq (eqb p s1); intros.
+    assert (p = s1). apply eqb_eq; try easy. subst. apply ha_sendp.
+  - case_eq (eqb p s2); intros.
+    assert (p = s2). apply eqb_eq; try easy. subst. apply ha_sendq.
+  - assert (p <> s1). apply eqb_neq; try easy. 
+    assert (p <> s2). apply eqb_neq; try easy.
+    apply ha_sendr with (n := 0) (s := o1) (g := o2); try easy.
+Qed.
+
+Lemma isgParts_xs : forall [s s' x o p],
+    isgParts p (g_send s s' x) ->
+    isgParts p (g_send s s' (o :: x)).
+Proof.
+  intros. inversion H. subst. 
+  constructor. 
+  subst. constructor.
+  subst. apply pa_sendr with (n := Nat.succ n) (s := s0) (g := g); try easy.
+Qed.
+
+Lemma ishParts_hxs : forall [p s1 s2 o1 xs0],
+    (ishParts p (gtth_send s1 s2 (o1 :: xs0)) -> False) ->
+    (ishParts p (gtth_send s1 s2 xs0) -> False).
+Proof.
+  intros. apply H.
+  inversion H0. subst. apply ha_sendp. apply ha_sendq.
+  subst. apply ha_sendr with (n := Nat.succ n) (s := s) (g := g); try easy.
+Qed.
+
+Lemma ishParts_n : forall [n p s s' xs s0 g],
+    (ishParts p (gtth_send s s' xs) -> False) ->
+    onth n xs = Some(s0, g) -> 
+    (ishParts p g -> False).
+Proof.  
+  induction n; intros; try easy.
+  - apply H. destruct xs; try easy. simpl in *. subst.
+    - case_eq (eqb p s); intros.
+      assert (p = s). apply eqb_eq; try easy. subst. apply ha_sendp.
+    - case_eq (eqb p s'); intros.
+      assert (p = s'). apply eqb_eq; try easy. subst. apply ha_sendq.
+    - assert (p <> s). apply eqb_neq; try easy. 
+      assert (p <> s'). apply eqb_neq; try easy.
+      apply ha_sendr with (n := 0) (s := s0) (g := g); try easy.
+  - destruct xs; try easy.
+    specialize(ishParts_hxs H); intros.
+    specialize(IHn p s s' xs s0 g). apply IHn; try easy.
+Qed.
+
+Lemma isgParts_x : forall [s s' x s0 g p],
+    isgParts p g -> 
+    isgParts p (g_send s s' (Some (s0, g) :: x)).
+Proof.
+    intros.
+    - case_eq (eqb p s); intros.
+      assert (p = s). apply eqb_eq; try easy. subst. apply pa_sendp.
+    - case_eq (eqb p s'); intros.
+      assert (p = s'). apply eqb_eq; try easy. subst. apply pa_sendq.
+    - assert (p <> s). apply eqb_neq; try easy. 
+      assert (p <> s'). apply eqb_neq; try easy.
+      apply pa_sendr with (n := 0) (s := s0) (g := g); try easy.
+Qed.
+
+Inductive isgParts_depth : fin -> part -> global -> Prop := 
+  | dpth_p : forall p q lis, isgParts_depth 0 p (g_send p q lis)
+  | dpth_q : forall p q lis, isgParts_depth 0 q (g_send p q lis)
+  | dpth_mu : forall n pt g, isgParts_depth n pt g -> isgParts_depth (S n) pt (g_rec g)
+  | dpth_c : forall p q pt s g lis n k, p <> pt -> q <> pt -> onth k lis = Some(s, g) -> isgParts_depth n pt g -> isgParts_depth (S n) pt (g_send p q lis).
+
+
+Lemma isgParts_depth_exists : forall r Gl,
+    isgParts r Gl -> exists n, isgParts_depth n r Gl.
+Proof.
+  induction Gl using global_ind_ref; intros; try easy.
+  inversion H0.
+  - subst. exists 0. constructor.
+  - subst. exists 0. constructor.
+  - subst. 
+    specialize(some_onth_implies_In n lis (s, g) H7); intros.
+    specialize(Forall_forall (fun u : option (sort * global) =>
+       u = None \/
+       (exists (s : sort) (g : global),
+          u = Some (s, g) /\
+          (isgParts r g -> exists n : fin, isgParts_depth n r g))) lis); intros.
+    destruct H2. specialize(H2 H). clear H H3.
+    specialize(H2 (Some (s, g)) H1).
+    destruct H2; try easy. destruct H. destruct H. destruct H. inversion H. subst. clear H.
+    specialize(H2 H8). destruct H2.
+    exists (S x1). apply dpth_c with (s := x) (g := x0) (k := n); try easy.
+  - inversion H. subst. specialize(IHGl H2). destruct IHGl. exists (S x). constructor. easy.
+Qed.
+
+Lemma isgParts_depth_back : forall G n r,
+      isgParts_depth n r G -> isgParts r G.
+Proof.
+  induction G using global_ind_ref; intros; try easy.
+  inversion H0. 
+  - subst. constructor.
+  - subst. constructor.
+  - subst. 
+    specialize(some_onth_implies_In k lis (s, g) H8); intros.
+    specialize(Forall_forall (fun u : option (sort * global) =>
+       u = None \/
+       (exists (s : sort) (g : global),
+          u = Some (s, g) /\
+          (forall (n : fin) (r : string),
+           isgParts_depth n r g -> isgParts r g))) lis); intros.
+    destruct H2. specialize(H2 H). clear H H3.
+    specialize(H2 (Some (s, g)) H1). destruct H2; try easy. destruct H. destruct H. destruct H.
+    inversion H. subst.
+    specialize(H2 n0 r H9). 
+    apply pa_sendr with (n := k) (s := x) (g := x0); try easy.
+  inversion H. subst.
+  - specialize(IHG n0 r H3). constructor. easy.
+Qed.
+
+
+Lemma subst_parts_helper : forall k0 xs s g0 r n0 lis m n g,
+      onth k0 xs = Some (s, g0) -> 
+      isgParts_depth n0 r g0 ->
+      Forall2
+       (fun u v : option (sort * global) =>
+        u = None /\ v = None \/
+        (exists (s : sort) (g0 g' : global),
+           u = Some (s, g0) /\ v = Some (s, g') /\ subst_global m n (g_rec g) g0 g')) xs lis -> 
+      Forall
+      (fun u : option (sort * global) =>
+       u = None \/
+       (exists (s : sort) (g : global),
+          u = Some (s, g) /\
+          (forall (m n k : fin) (r : string) (g0 g' : global),
+           isgParts_depth k r g' -> subst_global m n (g_rec g0) g' g -> isgParts_depth k r g))) lis -> 
+      exists g', onth k0 lis = Some (s, g') /\ isgParts_depth n0 r g'.
+Proof.
+  induction k0; intros; try easy.
+  - destruct xs; try easy.
+    simpl in H. subst. destruct lis; try easy. inversion H1. subst. clear H1. inversion H2. subst. clear H2.
+    clear H4 H7. destruct H5; try easy. destruct H. destruct H. destruct H. destruct H.
+    destruct H1. inversion H. subst.
+    destruct H3; try easy. destruct H1. destruct H1. destruct H1. inversion H1. subst.
+    specialize(H3 m n n0 r g x0 H0 H2).
+    exists x3. split; try easy.
+  - destruct xs; try easy. destruct lis; try easy. inversion H1. subst. clear H1. inversion H2. subst. clear H2.
+    specialize(IHk0 xs s g0 r n0 lis m n g). apply IHk0; try easy.
+Qed.
+
+Lemma subst_parts_depth : forall m n k r g g' Q,
+      subst_global m n (g_rec g) g' Q -> 
+      isgParts_depth k r g' -> 
+      isgParts_depth k r Q.
+Proof.
+  intros. revert H0 H. revert m n k r g g'.
+  induction Q using global_ind_ref; intros; try easy.
+  inversion H.
+  - subst. inversion H0; try easy.
+  - subst. inversion H0; try easy. 
+  - subst. inversion H0; try easy.
+  - inversion H. subst. inversion H0. 
+  - inversion H1. subst.
+    inversion H0. 
+    - subst. constructor.
+    - subst. constructor.
+    - subst. 
+      specialize(subst_parts_helper k0 xs s g0 r n0 lis m n g H10 H11 H7 H); intros. 
+      destruct H2. destruct H2.
+      apply dpth_c with (n := n0) (s := s) (g := x) (k := k0); try easy.
+  - inversion H. subst. inversion H0. 
+  - subst. inversion H0. subst.
+    constructor. specialize(IHQ m.+1 n.+1 n0 r g P). apply IHQ; try easy.
+Qed.
+
+
+Lemma part_after_step_helper : forall G1 q p x0,
+    gttTC G1 (gtt_send q p x0) -> 
+    (forall n : fin, exists m : fin, guardG n m G1) -> 
+    exists ys, gttTC (g_send q p ys) (gtt_send q p x0) /\ (forall n : fin, exists m : fin, guardG n m (g_send q p ys)).
+Proof.
+  intros. pinversion H; try easy. subst.
+  - exists xs. split. pfold. easy. easy.
+  - subst. specialize(guard_breakG G H0); intros.
+    destruct H3. destruct H3. destruct H4.
+    specialize(gtt_after_betaL (g_rec G) x (gtt_send q p x0)); intros.
+    assert(gttTC x (gtt_send q p x0)). 
+    apply H6; try easy. pfold. easy.
+    destruct H5. pinversion H7; try easy. subst. easy. subst. easy.
+    apply gttT_mon.
+    destruct H5. destruct H5. destruct H5. subst.
+    pinversion H7; try easy. subst. exists x3. split. pfold. easy. easy.
+    apply gttT_mon.
+    apply gttT_mon.
+Qed.
+
+Lemma part_break_s : forall G pt, 
+    isgPartsC pt G -> 
+    exists Gl, gttTC Gl G /\ isgParts pt Gl /\ (Gl = g_end \/ exists p q lis, Gl = g_send p q lis).
+Proof.
+  intros. pose proof H as H0.
+  unfold isgPartsC in H0. destruct H0. destruct H0.
+  rename x into Gl. destruct H1.
+  specialize(isgParts_depth_exists pt Gl H2); intros. destruct H3. rename x into n.
+  
+  clear H.
+  clear H2.
+  revert H3 H0 H1. revert G pt Gl.
+  induction n; intros; try easy.
+  - inversion H3. subst.
+    exists (g_send pt q lis). split. easy. split. constructor. right. exists pt. exists q. exists lis. easy.
+  - subst.
+    exists (g_send p pt lis). split. easy. split. constructor. right. exists p. exists pt. exists lis. easy.
+  - inversion H3. subst.
+    pinversion H0. subst.
+    specialize(subst_parts_depth 0 0 n pt g g Q H4 H2); intros.
+    apply IHn with (Gl := Q); try easy.
+    - intros. specialize(H1 n0). destruct H1. 
+      inversion H1. exists 0. constructor.
+      subst. exists m. specialize(subst_injG 0 0 (g_rec g) g Q Q0 H7 H4); intros. subst. easy.
+    apply gttT_mon.
+  - subst. 
+    exists (g_send p q lis). split. easy.
+    split.
+    apply pa_sendr with (n := k) (s := s) (g := g); try easy.
+    apply isgParts_depth_back with (n := n); try easy.
+    right. exists p. exists q. exists lis. easy.
+Qed.
+
+Lemma part_break_s2 : forall G pt, 
+    isgPartsC pt G -> 
+    exists Gl, gttTC Gl G /\ isgParts pt Gl /\ (forall n : fin, exists m : fin, guardG n m Gl) /\ (Gl = g_end \/ exists p q lis, Gl = g_send p q lis).
+Proof.
+  intros. pose proof H as H0.
+  unfold isgPartsC in H0. destruct H0. destruct H0.
+  rename x into Gl. destruct H1.
+  specialize(isgParts_depth_exists pt Gl H2); intros. destruct H3. rename x into n.
+  
+  clear H.
+  clear H2.
+  revert H3 H0 H1. revert G pt Gl.
+  induction n; intros; try easy.
+  - inversion H3. subst.
+    exists (g_send pt q lis). split. easy. split. constructor. split. easy. right. exists pt. exists q. exists lis. easy.
+  - subst.
+    exists (g_send p pt lis). split. easy. split. constructor. split. easy. right. exists p. exists pt. exists lis. easy.
+  - inversion H3. subst.
+    pinversion H0. subst.
+    specialize(subst_parts_depth 0 0 n pt g g Q H4 H2); intros.
+    apply IHn with (Gl := Q); try easy.
+    - intros. specialize(H1 n0). destruct H1. 
+      inversion H1. exists 0. constructor.
+      subst. exists m. specialize(subst_injG 0 0 (g_rec g) g Q Q0 H7 H4); intros. subst. easy.
+    apply gttT_mon.
+  - subst. 
+    exists (g_send p q lis). split. easy.
+    split.
+    apply pa_sendr with (n := k) (s := s) (g := g); try easy.
+    apply isgParts_depth_back with (n := n); try easy. split. easy.
+    right. exists p. exists q. exists lis. easy.
+Qed.
+
+Lemma part_break : forall G pt,
+    wfgC G -> 
+    isgPartsC pt G -> 
+    exists Gl, gttTC Gl G /\ isgParts pt Gl /\ (forall n : fin, exists m : fin, guardG n m Gl) /\ (Gl = g_end \/ exists p q lis, Gl = g_send p q lis).
+Proof.
+  intros. 
+  unfold isgPartsC in H0. destruct H0. destruct H0.
+  rename x into Gl. destruct H1.
+  specialize(isgParts_depth_exists pt Gl H2); intros. destruct H3. rename x into n.
+  
+  clear H.
+  clear H2.
+  revert H3 H0 H1. revert G pt Gl.
+  induction n; intros; try easy.
+  - inversion H3. subst.
+    exists (g_send pt q lis). split. easy. split. constructor. split. easy. right. exists pt. exists q. exists lis. easy.
+  - subst.
+    exists (g_send p pt lis). split. easy. split. constructor. split. easy. right. exists p. exists pt. exists lis. easy.
+  - inversion H3. subst.
+    pinversion H0. subst.
+    specialize(subst_parts_depth 0 0 n pt g g Q H4 H2); intros.
+    apply IHn with (Gl := Q); try easy.
+    - intros. specialize(H1 n0). destruct H1. 
+      inversion H1. exists 0. constructor.
+      subst. exists m. specialize(subst_injG 0 0 (g_rec g) g Q Q0 H7 H4); intros. subst. easy.
+    apply gttT_mon.
+  - subst. 
+    exists (g_send p q lis). split. easy.
+    split.
+    apply pa_sendr with (n := k) (s := s) (g := g); try easy.
+    apply isgParts_depth_back with (n := n); try easy. split. easy.
+    right. exists p. exists q. exists lis. easy.
+Qed.
+
 
 Lemma decidable_isgParts : forall G pt, decidable (isgParts pt G).
 Proof.
@@ -64,11 +436,84 @@ Proof.
     specialize(IHmultiS pt n1). apply IHmultiS; try easy.
 Qed.
 
+Lemma subst_after_incrG_b : forall G G' m n pt,
+    isgParts pt G' -> incr_freeG m n G = G' -> isgParts pt G.
+Proof.
+  induction G using global_ind_ref; intros; try easy.
+  - subst. inversion H; try easy.
+  - subst. inversion H; try easy.
+  - subst. 
+    inversion H0; try easy. subst. constructor. subst. constructor.
+    subst.
+    assert(exists g', onth n0 lis = Some(s, g') /\ g = incr_freeG m n g').
+    {
+      clear H8 H6 H4 H0 H. revert H7. revert lis.
+      induction n0; intros; try easy. destruct lis; try easy. simpl in H7.
+      destruct o; try easy. destruct p0; try easy. inversion H7. subst.
+      exists g0. easy.
+      destruct lis; try easy. specialize(IHn0 lis H7). apply IHn0; try easy.
+    }
+    destruct H1 as (g1,(Ha,Hb)). 
+    specialize(Forall_forall (fun u : option (sort * global) =>
+       u = None \/
+       (exists (s : sort) (g : global),
+          u = Some (s, g) /\
+          (forall (G' : global) (m n : fin) (pt : string),
+           isgParts pt G' -> incr_freeG m n g = G' -> isgParts pt g))) lis); intros.
+    destruct H1. specialize(H1 H). clear H2 H.
+    specialize(some_onth_implies_In n0 lis (s, g1) Ha); intros.
+    specialize(H1 (Some (s, g1)) H). destruct H1; try easy. 
+    destruct H1 as (s0,(g2,(Hd,He))). inversion Hd. subst.
+    specialize(He (incr_freeG m n g2) m n pt).
+    apply pa_sendr with (n := n0) (s := s0) (g := g2); try easy. 
+    apply He; try easy.
+  - subst. inversion H. subst.
+    specialize(IHG (incr_freeG m.+1 n G) (S m) n pt). 
+    constructor. apply IHG; try easy.
+Qed.
+
 Lemma subst_part_b : forall m n G G1 G2 pt,
     isgParts pt G2 -> 
     subst_global m n G G1 G2 -> 
     (isgParts pt G \/ isgParts pt G1).
-    
+Proof.
+  intros. revert H0 H. revert pt m n G G1.
+  induction G2 using global_ind_ref; intros; try easy.
+  - inversion H0.
+    - subst. left.
+      specialize(subst_after_incrG_b G (g_send p q lis) 0 n pt); intros.
+      apply H2; try easy.
+    - subst.
+      inversion H1.
+      - subst. right. constructor.
+      - subst. right. constructor.
+      subst.
+      revert H10 H9 H8 H5 H7 H. clear H0 H1.
+      revert p q lis pt m n G xs s g.
+      induction n0; intros; try easy.
+      - destruct lis; try easy. destruct xs; try easy. 
+        inversion H7. subst. clear H7. inversion H. subst. clear H.
+        simpl in H9. subst. 
+        destruct H3; try easy. destruct H as (s0,(g1,(g2,(Ha,(Hb,Hc))))). inversion Hb. subst.
+        destruct H2; try easy. destruct H as (s1,(g3,(Hd,He))). inversion Hd. subst.
+        specialize(He pt m n G g1 Hc H10).
+        destruct He. left. easy.
+        right. apply pa_sendr with (n := 0) (s := s1) (g := g1); try easy.
+      - destruct lis; try easy. destruct xs; try easy. 
+        inversion H7. subst. clear H7. inversion H. subst. clear H.
+        specialize(IHn0 p q lis pt m n G xs s g).
+        assert(isgParts pt G \/ isgParts pt (g_send p q xs)). apply IHn0; try easy.
+        destruct H. left. easy.
+        right. inversion H; try easy. subst. easy. subst. easy.
+        subst.
+        apply pa_sendr with (n := S n1) (s := s0) (g := g0); try easy.
+    - inversion H0. subst.
+      - specialize(subst_after_incrG_b G (g_rec G2) 0 n pt); intros.
+        left. apply H1; try easy.
+      - subst. inversion H. subst.
+        specialize(IHG2 pt (S m) (S n) G P H6 H3). 
+        destruct IHG2. left. easy. right. constructor. easy.
+Qed.
 
 
 Lemma part_betaG_b : forall G G' pt, multiS betaG G G' -> isgParts pt G' -> isgParts pt G.
@@ -79,13 +524,75 @@ Proof.
   induction H; intros.
   - inversion H. subst.
     specialize(subst_parts_depth 0 0 n pt G G y H0); intros.
-    specialize(isgParts_depth_back y n0 pt H2); intros. easy.
+    specialize(subst_part_b 0 0 (g_rec G) G y pt); intros.
+    specialize(isgParts_depth_back y n pt H1); intros.
+    constructor.
+    assert(isgParts pt (g_rec G) \/ isgParts pt G). apply H3; try easy.
+    destruct H5; try easy. inversion H5; try easy.
   - inversion H. subst.
-    inversion H1. subst.
-    specialize(subst_parts_depth 0 0 n0 pt G G y H2 H6); intros.
-    specialize(isgParts_depth_back y n0 pt H3); intros.
-    specialize(isgParts_depth_exists pt y H4); intros. destruct H5 as (n1, H5).
-    specialize(IHmultiS pt n1). apply IHmultiS; try easy.
+    specialize(IHmultiS pt n H1). clear H1 H0 H.
+    specialize(subst_part_b 0 0 (g_rec G) G y pt); intros. 
+    assert(isgParts pt (g_rec G) \/ isgParts pt G).
+    apply H; try easy. destruct H0; try easy. constructor; try easy.
+Qed.
+
+Lemma guardG_betaG : forall G G1,
+          (forall n : fin, exists m : fin, guardG n m G) -> 
+          multiS betaG G G1 -> 
+          (forall n : fin, exists m : fin, guardG n m G1).
+Proof.  
+  intros. revert n. revert H. 
+  induction H0; intros; try easy.
+  - inversion H. subst.
+    specialize(H0 n). destruct H0. inversion H0. subst. exists 0. constructor.
+    subst. specialize(subst_injG 0 0 (g_rec G) G y Q H3 H1); intros. subst. exists m. easy.
+  - revert n. apply IHmultiS. clear IHmultiS H0.
+    inversion H. subst. intros.
+    specialize(H1 n). destruct H1. inversion H1. exists 0. constructor.
+    subst. specialize(subst_injG 0 0 (g_rec G) G y Q H3 H0); intros. subst. exists m. easy.
+Qed.
+
+Lemma decidable_isgPartsC_helper : forall k lis s g ys xs,
+          onth k lis = Some (s, g) -> 
+          Forall2
+           (fun (u : option (sort * global)) (v : option (sort * gtt)) =>
+            u = None /\ v = None \/
+            (exists (s : sort) (g : global) (g' : gtt),
+               u = Some (s, g) /\ v = Some (s, g') /\ upaco2 gttT bot2 g g')) lis ys ->
+          Forall
+           (fun u : option (sort * global) =>
+            u = None \/
+            (exists (s : sort) (g : global),
+               u = Some (s, g) /\ (forall n : fin, exists m : fin, guardG n m g))) lis ->
+          Forall2
+           (fun (u : option (sort * global)) (v : option (sort * gtt)) =>
+            u = None /\ v = None \/
+            (exists (s : sort) (g : global) (g' : gtt),
+               u = Some (s, g) /\ v = Some (s, g') /\ upaco2 gttT bot2 g g')) xs ys ->
+          Forall
+           (fun u : option (sort * global) =>
+            u = None \/
+            (exists (s : sort) (g : global),
+               u = Some (s, g) /\ (forall n : fin, exists m : fin, guardG n m g))) xs -> 
+          exists g' g'', onth k ys = Some(s, g') /\ gttTC g g' /\
+          (forall n : fin, exists m : fin, guardG n m g) /\
+          onth k xs = Some(s, g'') /\ gttTC g'' g' /\ 
+          (forall n : fin, exists m : fin, guardG n m g'').
+Proof.
+  induction k; intros; try easy.
+  - destruct lis; try easy. destruct ys; try easy. destruct xs; try easy.
+    inversion H0. subst. clear H0. inversion H2. subst. clear H2.
+    inversion H1. subst. clear H1. inversion H3. subst. clear H3.
+    simpl in H. subst.
+    destruct H4; try easy. destruct H as (s1,(g1,(Ha,Hb))). inversion Ha. subst.
+    destruct H7; try easy. destruct H as (s2,(g2,(g3,(Hc,(Hd,He))))). inversion Hc. subst.
+    destruct H6; try easy. destruct H as (s3,(g4,(g5,(Hf,(Hg,Hh))))). inversion Hg. subst.
+    destruct H2; try easy. destruct H as (s4,(g6,(Hi,Hj))). inversion Hi. subst.
+    simpl. exists g5. exists g6. pclearbot. easy.
+  - destruct lis; try easy. destruct ys; try easy. destruct xs; try easy.
+    inversion H0. subst. clear H0. inversion H2. subst. clear H2.
+    inversion H1. subst. clear H1. inversion H3. subst. clear H3.
+    specialize(IHk lis s g ys xs). apply IHk; try easy.
 Qed.
 
 Lemma decidable_isgPartsC : forall G pt, wfgC G -> decidable (isgPartsC pt G).
@@ -108,10 +615,82 @@ Proof.
       destruct H0 as (T,(Hta,(Htb,Htc))).
       specialize(gttTC_after_subst (g_rec G) T (gtt_send pt q ys)); intros.
     - assert(gttTC T (gtt_send pt q ys)). apply H0; try easy. pfold. easy. clear H0.
-      specialize(part_betaG (g_rec G) T pt); intros.
-    
-Admitted.
-  
+      specialize(part_betaG_b (g_rec G) T pt); intros. apply H0; try easy.
+      destruct Htc. subst. pinversion H1; try easy. apply gttT_mon.
+      destruct H2 as (p1,(q1,(lis1,Hl))). subst. pinversion H1; try easy. subst.
+      constructor.
+      apply gttT_mon. apply gttT_mon. apply gttT_mon.
+    - subst. 
+      pinversion He; try easy. subst.
+      pinversion Ha. subst. constructor.
+      subst. clear H0 H1.
+      specialize(guard_breakG G Hc); intros.
+      destruct H0 as (T1,(Hta,(Htb,Htc))).
+      specialize(part_betaG_b (g_rec G) T1 pt); intros. apply H0; try easy.
+      clear H0.
+      specialize(gttTC_after_subst (g_rec G) T1 (gtt_send p pt ys)); intros.
+      assert(gttTC T1 (gtt_send p pt ys)). apply H0; try easy. pfold. easy.
+      clear H0. 
+      destruct Htc. subst. pinversion H1; try easy. apply gttT_mon.
+      destruct H0 as (p1,(q1,(lis1,Htc))). subst. pinversion H1; try easy. subst. 
+      constructor.
+      apply gttT_mon.
+      apply gttT_mon. apply gttT_mon.
+    - inversion H. 
+      - subst.
+        pinversion He; try easy. subst.
+        specialize(subst_parts_depth 0 0 n pt g g Q H2 H1); intros.
+        specialize(IHn G pt G' Q). apply IHn; try easy.
+        intros. specialize(Hf n0). destruct Hf. 
+        - inversion H4. subst. exists 0. constructor.
+        - subst. specialize(subst_injG 0 0 (g_rec g) g Q Q0 H6 H2); intros. subst.
+          exists m. easy.
+        apply gttT_mon.
+      - subst.
+        pinversion He; try easy. subst.
+        specialize(guard_cont Hf); intros.
+        pinversion Ha; try easy.
+        - subst.
+          specialize(guard_cont Hc); intros.
+          specialize(decidable_isgPartsC_helper k lis s g ys xs); intros.
+          assert(exists (g' : gtt) (g'' : global),
+       onth k ys = Some (s, g') /\
+       gttTC g g' /\
+       (forall n : fin, exists m : fin, guardG n m g) /\
+       onth k xs = Some (s, g'') /\ gttTC g'' g' /\ (forall n : fin, exists m : fin, guardG n m g'')).
+          apply H6; try easy. clear H6.
+          clear H8 H0 H7 H5. destruct H9 as (g1,(g2,(Hg,(Hh,(Hi,(Hj,(Hk,Hl))))))).
+          specialize(IHn g1 pt g2 g).
+          assert(isgParts pt g2). apply IHn; try easy.
+          apply pa_sendr with (n := k) (s := s) (g := g2); try easy.
+        - subst. clear H5 H6. clear Q.
+          specialize(guard_breakG G Hc); intros.
+          destruct H5 as (T1,(Hta,(Htb,Htc))).
+          specialize(gttTC_after_subst (g_rec G) T1 (gtt_send p q ys)); intros.
+          assert(gttTC T1 (gtt_send p q ys)). apply H5; try easy. pfold. easy.
+          clear H5. destruct Htc. subst. pinversion H6. apply gttT_mon.
+          destruct H5 as (p1,(q1,(lis1,Htc))). subst. pinversion H6. subst.
+          specialize(part_betaG_b (g_rec G) (g_send p q lis1) pt); intros. apply H5; try easy.
+          clear H5 Htb.
+          specialize(guardG_betaG (g_rec G) (g_send p q lis1)); intros.
+          assert(forall n : fin, exists m : fin, guardG n m (g_send p q lis1)). apply H5; try easy.
+          clear H5.
+          specialize(guard_cont H9); intros.
+          specialize(decidable_isgPartsC_helper k lis s g ys lis1); intros.
+          assert(exists (g' : gtt) (g'' : global),
+        onth k ys = Some (s, g') /\
+        gttTC g g' /\
+        (forall n : fin, exists m : fin, guardG n m g) /\
+        onth k lis1 = Some (s, g'') /\ gttTC g'' g' /\ (forall n : fin, exists m : fin, guardG n m g'')).
+          apply H10; try easy. clear H10.
+          destruct H11 as (g1,(g2,(Hg,(Hh,(Hi,(Hj,(Hk,Hl))))))).
+          specialize(IHn g1 pt g2 g).
+          assert(isgParts pt g2). apply IHn; try easy.
+          apply pa_sendr with (n := k) (s := s) (g := g2); try easy.
+      apply gttT_mon.
+      apply gttT_mon. 
+      apply gttT_mon.
+Qed.
   
   
   
